platform/cito/InvFacts.v
@@ -1,0 +1,17 @@
+Require Import Inv.
+Require Import Semantics.
+
+Set Implicit Arguments.
+
+Lemma make_triples_Word : forall pairs outs, length outs = length pairs -> map Word (make_triples pairs outs) = map fst pairs.
+  admit.
+Qed.
+
+Lemma make_triples_Forall_pair : forall pairs outs f, length outs = length pairs -> List.Forall f pairs -> List.Forall (fun x => f (Word x, ADTIn x)) (make_triples pairs outs).
+  admit.
+Qed.
+
+Lemma make_triples_ADTIn : forall pairs outs, length outs = length pairs -> map ADTIn (make_triples pairs outs) = map snd pairs.
+  admit.
+Qed.
+
