platform/cito/SepHints4.v
@@ -1,0 +1,15 @@
+Require Import AutoSep.
+Require Import List.
+
+Set Implicit Arguments.
+
+Definition locals_to_elim (_ : list string) := True.
+
+Lemma elim_locals : forall vars vs p, locals_to_elim vars -> locals vars vs 0 p ===> p =?> length vars.
+  admit.
+Qed.
+
+Definition hints_elim_locals : TacPackage.
+  prepare elim_locals tt.
+Defined.
+
